Fsub_Infrastructure.v
@@ -876,31 +876,31 @@ Proof with auto.
 Qed.
 
 
-(* Lemma open_ee_rec_expr : forall u e k,
-  expr e ->
-  e = open_ee_rec k u e.
-Proof with auto*.
-  intros u e k Hexpr. revert k.
-  induction Hexpr; intro k; simpl; f_equal; auto*;
-  try solve [
-    (** NEW: Something to deal with capture sets. *)
-    unfold open_ee in *; unfold open_ec in *;
-    pick fresh x;
-    eapply open_ee_rec_expr_aux with (j := 0) (v := exp_fvar x);
-    auto*;
-    eapply open_ee_rec_capt_aux with (j := 0) (C := {}C);
-    auto*
-  | unfold open_te in *;
-    pick fresh X;
-    eapply open_ee_rec_type_aux with (j := 0) (V := typ_fvar X);
-    auto*
-  ].
-Qed. *)
-
 Lemma open_ec_rec_expr : forall e c k,
   expr e ->
   e = open_ec_rec k c e.
 Proof with auto*.
+  intros e c k Ee. revert k.
+  induction Ee ; intro k ; simpl ; f_equal ; auto using open_tc_rec_type...
+  - pick fresh Z.
+    assert (open_ec (open_ee e1 Z) {}C = open_ec_rec k c (open_ec (open_ee e1 Z) {}C)). {
+      apply H1. fsetdec.
+    }    
+    unfold open_ee in H2.
+    rewrite <- open_ee_rec_expr in H2...
+    
+    admit.
+    admit.
+  - pick fresh Z.
+    assert (open_te e1 Z = open_ec_rec k c (open_te e1 Z)). {
+      apply H1. fsetdec.
+    }
+    rewrite <- open_te_expr with (U := Z) in H2...    
+    assert (expr (open_te e1 Z)). {
+      apply H0. fsetdec.
+    }
+    rewrite <- open_te_expr in H3.
+    admit. (* I am stuck here for now *)
 Admitted.
 
 Lemma open_ec_expr : forall e c,
